Trying to fix enq problem in generic fifos.

Fifo/GenericProofs.v
@@ -35,7 +35,9 @@ Section Proofs.
   
   Variable HsizePos : size <> 0.
   
-  Record myGenFifoR  (o_i o_s : RegsT) : Prop :=
+  Record myGenFifoR  (fifoRR fifoLR : RegsT -> RegsT -> Prop)
+         (fifoRegsL fifoRegsR : list (string * FullKind))
+         (o_i o_s : RegsT) : Prop :=
     {
       o_i1 : RegsT;
       o_i2 : RegsT;
@@ -78,11 +80,11 @@ Section Proofs.
                       existT _ GenericSpec.nlist implRegValR);
                      ((@GenericSpec.nonDetLenName ifcParamsR),
                       existT _ (SyntaxKind (Bit (lgSize + 1))) lenValR)];
-      Ho_iApp : o_i = o_i1 ++ o_i2;
-      HRegs1 : getKindAttr o_i1 = (fifoRegs HCorrectL);
-      HRegs2 : getKindAttr o_i2 = (fifoRegs HCorrectR);
-      HfifoR1 : (fifoR HCorrectL) o_i1 o_s1;
-      HfifoR2 : (fifoR HCorrectR) o_i2 o_s2;
+      Ho_iApp : o_i = o_i2 ++ o_i1;
+      HRegs1 : getKindAttr o_i1 = fifoRegsL;
+      HRegs2 : getKindAttr o_i2 = fifoRegsR;
+      HfifoR1 : fifoLR o_i1 o_s1;
+      HfifoR2 : fifoRR o_i2 o_s2;
       Ho_iNoDup1 : NoDup (map fst o_i);
       Ho_sNoDup1 : NoDup (map fst o_s);
     }.
@@ -90,14 +92,15 @@ Section Proofs.
 
   Ltac Record_destruct :=
     match goal with
-    | [H : myGenFifoR _ _ |- _] =>
+    | [H : myGenFifoR _ _ _ _ _ _ |- _] =>
       destruct H
     end.
 
   Goal FifoCorrect fifoImpl fifoSpec.
-    destruct HCorrectL, HCorrectR.
-    econstructor 1 with (fifoR := myGenFifoR)
-                        (fifoRegs := fifoRegs0 ++ fifoRegs).
+    (*destruct HCorrectL, HCorrectR.*)
+    econstructor 1 with (fifoR := myGenFifoR (fifoR HCorrectR) (fifoR HCorrectL)
+                                             (fifoRegs HCorrectL) (fifoRegs HCorrectR))
+                        (fifoRegs := (fifoRegs HCorrectL) ++ (fifoRegs HCorrectR)).
     all : unfold EffectfulRelation, EffectlessRelation, ActionWb,
           fifoImpl, fifoSpec, impl, spec,
           isEmpty, isFull, numFree, first, deq, enq, flush,
@@ -105,7 +108,7 @@ Section Proofs.
           GenericSpec.deq, GenericSpec.enq, GenericSpec.flush,
           DoubleFifo.isEmpty, DoubleFifo.isFull, DoubleFifo.numFree, DoubleFifo.first,
           DoubleFifo.deq, DoubleFifo.enq, DoubleFifo.flush.
-    all: intros; try Record_destruct; destruct HCorrectL, HCorrectR;
+    all: intros; try Record_destruct; try destruct HCorrectL, HCorrectR;
       cbn [CorrectDef.fifoRegs CorrectDef.fifoR] in *;
       unfold fifoSpecR, fifoSpecL, spec,  GenericSpec.enq, GenericSpec.deq,
       GenericSpec.first, GenericSpec.isEmpty,
@@ -151,24 +154,24 @@ Section Proofs.
          { clear; intros; f_equal; auto. }
          specialize (P0 _ _ _ e).
          do 2 rewrite wordToNat_natToWord in P0; [exact P0 |apply zero_lt_pow2 | | ].
-         --  specialize (wordBound _ x1) as P1; apply boundProofZ in P1.
-             unfold lgSize in *.
-             rewrite sizeSum at 1.
-             unfold size in P1.
-             unfold wordToNat in *; destruct x1; simpl in *; dest.
-             rewrite pow2_of_nat in H5.
-             rewrite <- (Z2Nat.id wordVal), <- Nat2Z.inj_lt in H5; auto.
-             apply (Nat.lt_le_trans _ (2 ^ (Nat.log2_up sizeL + 1))); auto.
-             apply pow2_le, plus_le_compat_r, Nat.log2_up_le_mono; lia.
-         --  specialize (wordBound _ x1) as P1; apply boundProofZ in P1.
-             unfold lgSize in *.
-             rewrite sizeSum at 1.
-             unfold size in P1.
-             unfold wordToNat in *; destruct x1; simpl in *; dest.
-             rewrite pow2_of_nat in H5.
-             rewrite <- (Z2Nat.id wordVal), <- Nat2Z.inj_lt in H5; auto.
-             apply (Nat.lt_le_trans _ (2 ^ (Nat.log2_up sizeL + 1))); auto.
-             apply pow2_le, plus_le_compat_r, Nat.log2_up_le_mono; lia.
+         -- specialize (wordBound _ x) as P1; apply boundProofZ in P1.
+            unfold lgSize in *.
+            rewrite sizeSum at 1.
+            unfold size in P1.
+            unfold wordToNat in *; destruct x; simpl in *; dest.
+            rewrite pow2_of_nat in H5.
+            rewrite <- (Z2Nat.id wordVal), <- Nat2Z.inj_lt in H5; auto.
+            apply (Nat.lt_le_trans _ (2 ^ (Nat.log2_up sizeL + 1))); auto.
+            apply pow2_le, plus_le_compat_r, Nat.log2_up_le_mono; lia.
+         -- specialize (wordBound _ x) as P1; apply boundProofZ in P1.
+            unfold lgSize in *.
+            rewrite sizeSum at 1.
+            unfold size in P1.
+            unfold wordToNat in *; destruct x; simpl in *; dest.
+            rewrite pow2_of_nat in H5.
+            rewrite <- (Z2Nat.id wordVal), <- Nat2Z.inj_lt in H5; auto.
+            apply (Nat.lt_le_trans _ (2 ^ (Nat.log2_up sizeL + 1))); auto.
+            apply pow2_le, plus_le_compat_r, Nat.log2_up_le_mono; lia.
        * symmetry; rewrite Nat.eqb_neq in *; intro; apply P; lia.
      + destruct Nat.eqb eqn:G0.
        * rewrite Nat.eqb_eq in G0; rewrite G0, diag; simpl; reflexivity.
@@ -196,7 +199,7 @@ Section Proofs.
       rewrite (Eqdep.EqdepTheory.UIP_refl _ _ x1); simpl.
       destruct wltu eqn:G.
       + rewrite wltu_lt in G.
-        destruct (wltu ($ (wordToNat x2)) _) eqn:G0.
+        destruct (wltu ($ (wordToNat x0)) _) eqn:G0.
         * unfold lgSize, ZeroExtendTruncLsb.
           destruct lt_dec.
           -- rewrite evalExpr_castBits, nat_cast_eq_rect.
@@ -204,11 +207,11 @@ Section Proofs.
              rewrite (f_equal_dep (fun n : nat => word n)
                                      (fun n =>
                                         (wconcat (wzero (Nat.log2_up size + 1
-                                                    - (Nat.log2_up sizeL + 1))) x2))
+                                                    - (Nat.log2_up sizeL + 1))) x0))
                                      (ZeroExtendTruncLsb_subproof l)).
                 arithmetizeWord.
                 unfold wordToNat, lgSize, size; rewrite Z2Nat.id; auto.
-                specialize (Word.wordBound _ x2) as P; apply boundProofZ in P; dest; auto.
+                specialize (Word.wordBound _ x0) as P; apply boundProofZ in P; dest; auto.
           -- assert (Nat.log2_up size = Nat.log2_up sizeL) as P.
              { rewrite Nat.nlt_ge in n.
                destruct (le_lt_or_eq _ _ n); [|unfold size in *; lia].
@@ -222,7 +225,7 @@ Section Proofs.
              simpl.
              rewrite evalExpr_castBits, nat_cast_eq_rect.
              specialize (f_equal_dep (fun n : nat => word n)
-                                     (fun n => $(wordToNat x2))
+                                     (fun n => $(wordToNat x0))
                                      (ZeroExtendTruncLsb_subproof0 n)) as P0.
              simpl in *.
              rewrite natToWord_wordToNat in P0; rewrite P0.
@@ -230,7 +233,7 @@ Section Proofs.
              rewrite diag, Nat.add_0_r.
              repeat rewrite natToWord_wordToNat.
              apply eq_wordVal; simpl; rewrite Z.mod_small; auto.
-             specialize (wordBound _ x2) as P1; apply boundProofZ in P1; dest; auto.
+             specialize (wordBound _ x0) as P1; apply boundProofZ in P1; dest; auto.
         * exfalso.
           rewrite wltu_ge, sizeSum, app_length, <- Nat.nlt_ge in G0; apply G0.
           repeat rewrite wordToNat_natToWord.
@@ -245,9 +248,9 @@ Section Proofs.
                [apply log2_up_pow2|].
              apply Nat.pow_lt_mono_r; lia.
           -- apply (Nat.lt_le_trans _ (2 ^ ((Nat.log2_up sizeL) + 1))).
-             ++ specialize (wordBound _ x2) as P; apply boundProofZ in P; dest.
+             ++ specialize (wordBound _ x0) as P; apply boundProofZ in P; dest.
                 unfold lgSize, size in H5.
-                unfold wordToNat in *; destruct x2; simpl in *; dest.
+                unfold wordToNat in *; destruct x0; simpl in *; dest.
                 rewrite pow2_of_nat in H5.
                 rewrite <- (Z2Nat.id wordVal), <- Nat2Z.inj_lt in H5; auto.
              ++ unfold lgSize; rewrite sizeSum.
@@ -347,34 +350,36 @@ Section Proofs.
       + goal_consumer1.
         rewrite (Eqdep.EqdepTheory.UIP_refl _ _ x0).
         apply functional_extensionality_dep.
-        intros; fin_dep_destruct x.
+        intros; fin_dep_destruct x1.
         * simpl.
-          destruct implRegValR, implRegValL, x8; simpl; auto.
+          destruct implRegValR, implRegValL, x; simpl; auto.
         * fin_dep_destruct y; auto; simpl.
-          destruct implRegValR, implRegValL, x8; simpl; auto.
+          destruct implRegValR, implRegValL, x; simpl; auto.
     - hyp_consumer.
       goal_consumer2.
     - hyp_consumer.
-      + goal_consumer1.
-        * rewrite (Eqdep.EqdepTheory.UIP_refl _ _ x0).
-          apply functional_extensionality_dep.
-          intros; fin_dep_destruct x.
-          -- simpl.
-             destruct implRegValR, implRegValL, x8; simpl; auto.
-          -- fin_dep_destruct y; auto; simpl.
-             destruct implRegValR, implRegValL, x8; simpl; auto.
-        * econstructor 1; auto; normalize_key_concl; simpl;
-            try intro; repeat rewrite doUpdRegs_preserves_keys; auto.
-          -- admit.
-          -- admit.
-          -- admit.
-          -- admit.
+      goal_consumer1.
+      + rewrite (Eqdep.EqdepTheory.UIP_refl _ _ x0).
+        apply functional_extensionality_dep.
+        intros; fin_dep_destruct x1.
+        * simpl.
+          destruct implRegValR, implRegValL, x; simpl; auto.
+        * fin_dep_destruct y; auto; simpl.
+          destruct implRegValR, implRegValL, x; simpl; auto.
+      + econstructor 1; normalize_key_concl; simpl;
+            try intro; repeat rewrite doUpdRegs_preserves_keys; eauto.
+        * rewrite doUpdRegs_DisjKey; try solve_keys; auto.
+        * rewrite doUpdReg_preserves_getKindAttr; auto.
+        * rewrite doUpdRegs_DisjKey; try solve_keys.
+          exact HfifoR1.
+        * repeat rewrite doUpdReg_nil in *; rewrite doUpdRegs_nil in *.
+          exact HdoUpdRegsR.
     - hyp_consumer.
       goal_consumer2.
     - hyp_consumer.
-      goal_consumer1; rewrite (Eqdep.EqdepTheory.UIP_refl _ _ x0) in *.
-      + simpl.
-        destruct weq; subst; simpl.
+      rewrite (Eqdep.EqdepTheory.UIP_refl _ _ x0) in *.
+      goal_consumer1; simpl.
+      + destruct weq; subst; simpl.
         * destruct wltu eqn:G; auto.
           rewrite wltu_ge in G.
           destruct (le_lt_or_eq _ _ G).
@@ -392,32 +397,32 @@ Section Proofs.
                 ++ apply Nat.pow_lt_mono_r; lia.
                 ++ apply (Nat.le_trans _ sizeL); try lia; apply log2_up_pow2.
                 ++ apply Nat.pow_lt_mono_r; lia.
-        * destruct weq; simpl. 
+        * destruct weq; simpl.
           -- destruct wltu eqn:G.
              ++ exfalso.
                 apply neq_wordVal in n; apply n; simpl.
                 unfold wordToNat in e.
-                destruct x10; simpl in *.
-                arithmetizeWord; simpl in H6.
+                destruct x; simpl in *.
+                arithmetizeWord; simpl in H10.
                 rewrite Zmod_0_l; auto.
-                rewrite Zmod_0_l, pow2_of_nat, <- mod_Zmod in H6;
+                rewrite Zmod_0_l, pow2_of_nat, <- mod_Zmod in H10;
                   [|specialize (zero_lt_pow2 (lgSize + 1)) as TMP; lia].
-                rewrite Nat.mod_small in H6;
-                  [rewrite Z2Nat.id in H6|]; try lia.
+                rewrite Nat.mod_small in H10;
+                  [rewrite Z2Nat.id in H10|]; try lia.
                 unfold lgSize; rewrite sizeSum.
                 dest.
-                unfold lgSize, size in H10, H13.
-                rewrite pow2_of_nat in H13, H10.
+                unfold lgSize, size in H11, H13.
+                rewrite pow2_of_nat in H11, H13.
                 rewrite <- (Z2Nat.id wordVal) in H13; auto.
-                rewrite <- (Z2Nat.id wordVal0) in H10; auto.
-                rewrite <- Nat2Z.inj_lt in H10, H13.
+                rewrite <- (Z2Nat.id wordVal0) in H11; auto.
+                rewrite <- Nat2Z.inj_lt in H11, H13.
                 apply (Nat.lt_le_trans _ (2 ^ (Nat.log2_up sizeL + 1))),
                 Nat.pow_le_mono_r, plus_le_compat_r, Nat.log2_up_le_mono; lia.
              ++ rewrite Nat.eqb_eq.
-                arithmetizeWord; simpl in H5.
-                rewrite Zmod_0_l, pow2_of_nat, <- mod_Zmod in H5;
+                arithmetizeWord; simpl in H6.
+                rewrite Zmod_0_l, pow2_of_nat, <- mod_Zmod in H6;
                   [|specialize (zero_lt_pow2 (lgSize + 1)) as TMP; lia].
-                rewrite Nat.mod_small in H5; try lia.
+                rewrite Nat.mod_small in H6; try lia.
                 unfold lgSize; rewrite sizeSum.
                 apply (Nat.le_lt_trans _ sizeL); [lia|].
                 apply (Nat.le_lt_trans _ (sizeL + sizeR)); [lia|].
@@ -436,41 +441,262 @@ Section Proofs.
                 rewrite Nat.eqb_neq in *; intro; apply G; lia.
       + econstructor 1; auto; normalize_key_concl; simpl;
           try intro; repeat rewrite doUpdRegs_preserves_keys; auto; simpl in *.
-        * instantiate (1 := (if
-                                negb
-                                  (getBool (weq x10 $ (0))
-                                   || (Datatypes.length implRegValL =? sizeL)%nat)
-                              then GenericSpec.snocInBound val implRegValL
-                              else implRegValL)).
-          admit.
-        * instantiate (1 := implRegValR); auto.
-        * instantiate (1 := x10).
-          instantiate (1 := nonDetEmpValR).
-          admit.
-        * admit.
-        * admit.
-        * instantiate (1 := nonDetEmpValL).
-          admit.
-        * instantiate (1 := lenValR).
-          admit.
+        6 : { revert HdoUpdRegsR.
+              doUpdRegs_red; intro.
+              destruct String.eqb eqn:G in HdoUpdRegsR.
+              - unfold GenericSpec.listName in G.
+                rewrite String.eqb_eq, append_remove_prefix in G.
+                discriminate.
+              - destruct String.eqb eqn:G0 in HdoUpdRegsR.
+                + exfalso.
+                  rewrite String.eqb_eq in G0;
+                    unfold GenericSpec.nonDetLenName, GenericSpec.listName in *.
+                  apply append_remove_prefix in G0; discriminate.
+                + apply HdoUpdRegsR.
+        }
+        6 : { rewrite doUpdRegs_DisjKey; [|solve_keys].
+              apply HfifoR2.
+        }
+        * unfold GenericSpec.snocInBound, size.
+          (* instantiate (1 := (if negb *)
+          (*                         (getBool (weq x $ (0)) *)
+          (*                          || (Datatypes.length implRegValL =? sizeL)%nat) *)
+          (*                     then *)
+          (*                       if Datatypes.length implRegValL <? sizeL *)
+          (*                       then snoc val implRegValL *)
+          (*                       else implRegValL *)
+          (*                     else implRegValL)). *)
+          destruct weq; simpl; auto.
+          destruct Nat.eqb eqn:G; simpl; auto.
+          destruct Nat.ltb eqn:G0; auto.
+          rewrite Nat.eqb_neq in G.
+          rewrite snoc_rapp, app_length; simpl; lia.
+        * (* instantiate (1 := implRegValR); *) auto.
+        * (* instantiate (1 := x). *)
+          (* instantiate (1 := nonDetEmpValR). *)
+          repeat f_equal.
+          -- repeat destruct weq; simpl; auto; subst.
+             ++ destruct wltu eqn:G.
+                ** exfalso.
+                   apply n; rewrite wordToNat_natToWord; auto.
+                   apply zero_lt_pow2.
+                ** exfalso.
+                   rewrite wltu_ge in G.
+                   do 2 rewrite wordToNat_natToWord in G; try apply zero_lt_pow2.
+                   --- destruct (le_lt_or_eq _ _ G); [lia|].
+                       rewrite H0 in n; apply n; reflexivity.
+                   --- unfold lgSize, size.
+                       apply (Nat.le_lt_trans _ sizeL); [lia|].
+                       apply (Nat.le_lt_trans _ (2 ^ (Nat.log2_up sizeL)));
+                         [apply log2_up_pow2|apply Nat.pow_lt_mono_r;lia].
+                   --- unfold lgSize, size.
+                       apply (Nat.le_lt_trans _ sizeL); [lia|].
+                       apply (Nat.le_lt_trans _ (2 ^ (Nat.log2_up sizeL)));
+                         [apply log2_up_pow2|apply Nat.pow_lt_mono_r;lia].
+             ++ destruct wltu eqn:G.
+                ** exfalso.
+                   clear HdoUpdRegsR.
+                   apply neq_wordVal in n; apply n.
+                   unfold wordToNat in e.
+                   arithmetizeWord; simpl in *.
+                   rewrite Zmod_0_l.
+                   rewrite Zmod_0_l, pow2_of_nat, <- mod_Zmod in H10;
+                     [|specialize (zero_lt_pow2 (lgSize + 1)) as TMP; lia].
+                   rewrite Nat.mod_small in H10;
+                     [rewrite Z2Nat.id in H10|]; try lia.
+                   unfold lgSize; rewrite sizeSum.
+                   dest.
+                   unfold lgSize, size in H11, H13.
+                   rewrite pow2_of_nat in H11, H13.
+                   rewrite <- (Z2Nat.id wordVal) in H13; auto.
+                   rewrite <- (Z2Nat.id wordVal0) in H11; auto.
+                   rewrite <- Nat2Z.inj_lt in H11, H13.
+                   apply (Nat.lt_le_trans _ (2 ^ (Nat.log2_up sizeL + 1))),
+                   Nat.pow_le_mono_r, plus_le_compat_r, Nat.log2_up_le_mono; lia.
+                ** destruct Nat.eqb eqn:G0; simpl; auto.
+                   exfalso.
+                   rewrite Nat.eqb_neq in G0; apply G0.
+                   arithmetizeWord; simpl in H10.
+                   rewrite Zmod_0_l, pow2_of_nat, <- mod_Zmod in H10;
+                     [|specialize (zero_lt_pow2 (lgSize + 1)) as TMP; lia].
+                   rewrite <- (Z2Nat.id 0) in H10; [|lia].
+                   apply Nat2Z.inj in H10.
+                   rewrite Nat.mod_small in H10; try lia.
+                   unfold lgSize; rewrite sizeSum.
+                   apply (Nat.le_lt_trans _ sizeL); [lia|].
+                   apply (Nat.le_lt_trans _ (sizeL + sizeR)); [lia|].
+                   apply (Nat.le_lt_trans _ (2 ^ (Nat.log2_up (sizeL + sizeR))));
+                     [apply log2_up_pow2| apply Nat.pow_lt_mono_r; lia].
+             ++ rewrite app_length, sizeSum.
+                destruct Nat.eqb eqn:G; simpl.
+                ** rewrite Nat.eqb_eq in G; rewrite G in *.
+                   exfalso.
+                   rewrite diag in *; simpl in *.
+                   destruct wltu eqn:G0 in n0; [|apply n0; reflexivity].
+                   rewrite wltu_lt, wordToNat_natToWord in G0; [lia |apply zero_lt_pow2].
+                ** destruct (Nat.eqb (_ + _) _) eqn:G0; simpl.
+                   --- exfalso.
+                       rewrite Nat.eqb_eq in G0.
+                       rewrite Nat.eqb_neq in G.
+                       lia.
+                   --- unfold GenericSpec.snocInBound; rewrite sizeSum, app_length.
+                       destruct Nat.ltb eqn:G1.
+                       +++ destruct (Nat.ltb (length implRegValL)) eqn:G2.
+                           *** repeat rewrite snoc_rapp.
+                               rewrite app_assoc; reflexivity.
+                           *** exfalso.
+                               unfold size in G2.
+                               rewrite Nat.ltb_ge in G2.
+                               rewrite Nat.eqb_neq in G.
+                               lia.
+                       +++ exfalso.
+                           rewrite Nat.eqb_neq in G0.
+                           rewrite Nat.ltb_ge in G1.
+                           lia.
+          -- destruct wltu eqn:G.
+             ++ destruct (wltu _ ($ (_ - length (if (negb _) then _ else _)))) eqn:G0; auto.
+                destruct weq in G0; simpl in *; [rewrite G0 in *; discriminate|].
+                destruct Nat.eqb eqn:G1 in G0; simpl in *; [rewrite G0 in *; discriminate|].
+                rewrite wltu_lt in G.
+                rewrite wltu_ge in G0.
+                unfold GenericSpec.snocInBound in G0.
+                destruct Nat.ltb eqn:G2; [| lia].
+                rewrite snoc_rapp, app_length in G0; simpl in *.
+                destruct weq; simpl; [contradiction|].
+                rewrite G1; simpl.
+                unfold GenericSpec.snocInBound, size; setoid_rewrite G2.
+                rewrite Nat.eqb_neq, Nat.ltb_lt in *.
+                rewrite snoc_rapp, app_length; simpl.
+                rewrite wordToNat_natToWord in G0, G.
+                ** destruct (le_lt_or_eq _ _ G0); [|rewrite H0 in *; reflexivity].
+                   exfalso.
+                   apply lt_le_S in H0.
+                   rewrite Nat.add_1_r, minus_Sn_m, Nat.sub_succ in H0; lia.
+                ** unfold lgSize, size.
+                   apply (Nat.le_lt_trans _ (2^ (Nat.log2_up sizeL)));
+                     [|apply Nat.pow_lt_mono_r; lia].
+                   apply (Nat.le_trans _ sizeL); [lia |apply log2_up_pow2].
+                ** unfold lgSize, size.
+                   apply (Nat.le_lt_trans _ (2^ (Nat.log2_up sizeL)));
+                     [|apply Nat.pow_lt_mono_r; lia].
+                   apply (Nat.le_trans _ sizeL); [lia |apply log2_up_pow2].
+             ++ rewrite wltu_ge in G.
+                destruct wltu eqn:G0; simpl.
+                ** exfalso.
+                   unfold GenericSpec.snocInBound, size in G0.
+                   rewrite wltu_lt in G0.
+                   destruct weq in G0; simpl in *; [lia|].
+                   destruct Nat.eqb eqn:G1 in G0; simpl in *; [lia|].
+                   destruct Nat.ltb eqn:G2 in G0; [|lia].
+                   rewrite snoc_rapp, app_length in G0; simpl in *.
+                   specialize (Nat.le_lt_trans _ _ _ G G0) as P.
+                   do 2 rewrite wordToNat_natToWord in P; [lia| | | ];
+                        unfold lgSize, size;
+                        apply (Nat.le_lt_trans _ (2^ (Nat.log2_up sizeL)));
+                        try (apply Nat.pow_lt_mono_r; lia);
+                        apply (Nat.le_trans _ sizeL); try lia; apply log2_up_pow2.
+                ** rewrite wltu_ge in G0.
+                   destruct weq; simpl in *; auto.
+                   destruct Nat.eqb eqn:G1; simpl in *; auto.
+                   unfold GenericSpec.snocInBound.
+                   destruct Nat.ltb eqn:G2; auto.
+                   exfalso.
+                   rewrite Nat.ltb_lt in G2.
+                   admit.
+        * rewrite doUpdReg_preserves_getKindAttr; auto.
+        * rewrite doUpdRegs_DisjKey; try solve_keys; auto.
+        (* * repeat rewrite doUpdReg_nil in *. *)
+        (*   instantiate (1 := nonDetEmpValL). *)
+        (*   unfold oneUpdReg in HdoUpdRegsR; simpl in *. *)
+        (*   unfold GenericSpec.listName, GenericSpec.nonDetLenName, *)
+        (*   GenericSpec.nonDetEmptyName in *. *)
+        (*   rewrite String.eqb_refl in *. *)
+        (*   repeat (destruct String.eqb eqn:G in HdoUpdRegsR; *)
+        (*           [rewrite String.eqb_eq, append_remove_prefix in G; discriminate| clear G]). *)
+        (*   simpl in *. *)
+        (*   apply HdoUpdRegsR. *)
+        (* * rewrite doUpdRegs_DisjKey; try solve_keys; auto. *)
+        (*   exact HfifoR2. *)
     - hyp_consumer.
       goal_consumer2.
-    - hyp_consumer.
-      goal_consumer1.
-      + econstructor 1; auto; normalize_key_concl; simpl;
-          try intro; repeat rewrite doUpdRegs_preserves_keys; auto; simpl in *;
-            goal_consumer2.
-        * instantiate (1 := implRegValL); simpl; auto.
-        * admit.
-        * instantiate (1 := lenValL).
-          simpl.
+    - unfold GenericSpec.listName, GenericSpec.nonDetLenName in *.
+      hyp_consumer.
+      goal_consumer1; auto.
+      + econstructor 1; normalize_key_concl;
+          try intro; repeat rewrite doUpdRegs_preserves_keys; auto.
+        * instantiate (1 := nil); simpl; lia.
+        * instantiate (1 := nil); simpl; lia.
+        * instantiate (1 := (if wltu lenValL $ (sizeL - Datatypes.length implRegValL)
+                             then $ (wordToNat lenValL)
+                             else $ (sizeL - Datatypes.length implRegValL))).
+          rewrite orb_true_r.
+          repeat f_equal; simpl.
+          rewrite Nat.sub_0_r.
+          destruct wltu eqn:G.
+          -- rewrite wltu_lt in G.
+             destruct wltu eqn:G0; repeat rewrite natToWord_wordToNat in *; auto.
+             exfalso.
+             rewrite wltu_ge in G0.
+             specialize (Nat.le_lt_trans _ _ _ G0 G) as P.
+             do 2 rewrite wordToNat_natToWord in P; try lia;
+                  unfold lgSize, size;
+                  apply (Nat.le_lt_trans _ (2^ (Nat.log2_up sizeL)));
+                  try (apply Nat.pow_lt_mono_r; lia);
+                  try (apply (Nat.le_trans _ sizeL); [lia |apply log2_up_pow2]).
+          -- clear G; destruct wltu eqn:G;
+              [rewrite wordToNat_natToWord; auto;
+               unfold lgSize, size;
+                 apply (Nat.le_lt_trans _ (2^ (Nat.log2_up sizeL)));
+                 try (apply Nat.pow_lt_mono_r; lia);
+                 try (apply (Nat.le_trans _ sizeL); [lia |apply log2_up_pow2])|].
+            rewrite wltu_ge in G.
+            destruct (le_lt_or_eq _ _ G).
+            ++ exfalso.
+               do 2 rewrite wordToNat_natToWord in H13; try lia;
+                    unfold lgSize, size;
+                    apply (Nat.le_lt_trans _ (2^ (Nat.log2_up sizeL)));
+                    try (apply Nat.pow_lt_mono_r; lia);
+                    try (apply (Nat.le_trans _ sizeL); [lia |apply log2_up_pow2]).
+            ++  do 2 rewrite wordToNat_natToWord in H13; try rewrite H13 at 2; try lia; auto;
+                     unfold lgSize, size;
+                     apply (Nat.le_lt_trans _ (2^ (Nat.log2_up sizeL)));
+                     try (apply Nat.pow_lt_mono_r; lia);
+                     try (apply (Nat.le_trans _ sizeL); [lia |apply log2_up_pow2]).
+        * rewrite doUpdRegs_DisjKey.
+          -- rewrite doUpdReg_preserves_getKindAttr; auto.
+          -- intro; rewrite doUpdRegs_preserves_keys; revert k; fold (DisjKey x0 o_i1).
+             solve_keys.
+        * rewrite doUpdReg_preserves_getKindAttr; auto.
+          -- rewrite doUpdRegs_DisjKey; auto.
+             solve_keys.
+          -- rewrite doUpdRegs_preserves_keys; auto.
+          -- rewrite doUpdRegs_DisjKey; auto.
+             solve_keys.
+        * rewrite doUpdRegs_DisjKey;
+            [|intro; rewrite doUpdRegs_preserves_keys; revert k; fold (DisjKey x0 o_i1);
+              solve_keys].
+          revert HdoUpdRegsR0.
+          doUpdRegs_red; intro.
+          destruct String.eqb eqn:G in HdoUpdRegsR0.
+          -- rewrite String.eqb_eq in G.
+             destruct String.eqb eqn:G0 in G;
+               [rewrite String.eqb_eq, append_remove_prefix in G0; discriminate
+               |rewrite append_remove_prefix in G; discriminate].
+          -- clear G.
+             destruct String.eqb eqn:G in HdoUpdRegsR0;
+               [rewrite String.eqb_eq, append_remove_prefix in G; discriminate|].
           admit.
-        * admit.
-        * admit.
-        * admit.
-        * admit.
-        * admit.
-        * admit.
+        * rewrite (@doUpdRegs_DisjKey o_i2 x7); [|solve_keys].
+          revert HdoUpdRegsR; doUpdRegs_red; intro.
+          destruct String.eqb eqn:G.
+          -- rewrite String.eqb_eq in G.
+             destruct String.eqb eqn:G0 in G;
+               [rewrite String.eqb_eq, append_remove_prefix in G0; discriminate
+               |rewrite append_remove_prefix in G; discriminate].
+          -- clear G.
+             destruct String.eqb eqn:G in HdoUpdRegsR;
+               [rewrite String.eqb_eq, append_remove_prefix in G; discriminate|].
+             apply HdoUpdRegsR.
     - hyp_consumer.
       goal_consumer2.
       Unshelve.
